src/ocaml/extraction/Typ.ml
@@ -1,3 +1,5 @@
+open Eqtype
+open Ssrnat
 
 type typ =
 | Tuint of int
@@ -8,3 +10,16 @@ type typ =
 let sizeof_typ = function
 | Tuint w -> w
 | Tsint w -> w
+
+(** val typ_eqn : typ -> typ -> bool **)
+
+let typ_eqn x y =
+  match x with
+  | Tuint wx ->
+    (match y with
+     | Tuint wy -> eq_op nat_eqType (Obj.magic wx) (Obj.magic wy)
+     | Tsint _ -> false)
+  | Tsint wx ->
+    (match y with
+     | Tuint _ -> false
+     | Tsint wy -> eq_op nat_eqType (Obj.magic wx) (Obj.magic wy))
