src/ocaml/extraction/Typ.mli
@@ -1,6 +1,10 @@
+open Eqtype
+open Ssrnat
 
 type typ =
 | Tuint of int
 | Tsint of int
 
 val sizeof_typ : typ -> int
+
+val typ_eqn : typ -> typ -> bool
