src/ocaml/extraction/TypEnv.ml
@@ -1,9 +1,13 @@
 open Bool
+open Datatypes
 open FMaps
+open List0
 open Typ
 open Var
+open Ssreflect
 
 type __ = Obj.t
+let __ = let rec f _ = Obj.repr f in Obj.repr f
 
 module type TypEnv =
  sig
@@ -51,6 +55,468 @@ module type TypEnv =
   val vtyp : SE.t -> env -> typ
 
   val vsize : SE.t -> env -> int
+
+  val eequal : env -> env -> bool
+ end
+
+module TypEnvLemmas =
+ functor (TE:TypEnv) ->
+ struct
+  module F =
+   struct
+    (** val eqb : TE.SE.t -> TE.SE.t -> bool **)
+
+    let eqb x y =
+      if TE.E.eq_dec x y then true else false
+
+    (** val coq_In_dec : 'a1 TE.t -> TE.key -> bool **)
+
+    let coq_In_dec m x =
+      let b = TE.mem x m in if b then true else false
+   end
+
+  module OP =
+   struct
+    module ME = OrderedType.OrderedTypeFacts(TE.E)
+
+    module O = OrderedType.KeyOrderedType(TE.E)
+
+    module P =
+     struct
+      module F =
+       struct
+        (** val eqb : TE.SE.t -> TE.SE.t -> bool **)
+
+        let eqb x y =
+          if TE.E.eq_dec x y then true else false
+
+        (** val coq_In_dec : 'a1 TE.t -> TE.key -> bool **)
+
+        let coq_In_dec m x =
+          let b = TE.mem x m in if b then true else false
+       end
+
+      (** val uncurry : ('a1 -> 'a2 -> 'a3) -> ('a1 * 'a2) -> 'a3 **)
+
+      let uncurry f p =
+        f (fst p) (snd p)
+
+      (** val of_list : (TE.key * 'a1) list -> 'a1 TE.t **)
+
+      let of_list l =
+        fold_right (uncurry TE.add) TE.empty l
+
+      (** val to_list : 'a1 TE.t -> (TE.key * 'a1) list **)
+
+      let to_list =
+        TE.elements
+
+      (** val fold_rec :
+          (TE.key -> 'a1 -> 'a2 -> 'a2) -> 'a2 -> 'a1 TE.t -> ('a1 TE.t -> __
+          -> 'a3) -> (TE.key -> 'a1 -> 'a2 -> 'a1 TE.t -> 'a1 TE.t -> __ ->
+          __ -> __ -> 'a3 -> 'a3) -> 'a3 **)
+
+      let fold_rec f i m hempty hstep =
+        let f0 = uncurry f in
+        let l = rev (TE.elements m) in
+        let hstep' = fun k e a m' m'' x ->
+          hstep (fst (k, e)) (snd (k, e)) a m' m'' __ __ __ x
+        in
+        let rec f1 l0 hstep'0 m0 =
+          match l0 with
+          | [] -> hempty m0 __
+          | y :: l1 ->
+            let (a, b) = y in
+            hstep'0 a b (fold_right f0 i l1) (of_list l1) m0 __ __ __
+              (f1 l1 (fun k0 e0 a0 m' m'' _ _ _ x ->
+                hstep'0 k0 e0 a0 m' m'' __ __ __ x) (of_list l1))
+        in f1 l (fun k e a m' m'' _ _ _ x -> hstep' k e a m' m'' x) m
+
+      (** val fold_rec_bis :
+          (TE.key -> 'a1 -> 'a2 -> 'a2) -> 'a2 -> 'a1 TE.t -> ('a1 TE.t ->
+          'a1 TE.t -> 'a2 -> __ -> 'a3 -> 'a3) -> 'a3 -> (TE.key -> 'a1 ->
+          'a2 -> 'a1 TE.t -> __ -> __ -> 'a3 -> 'a3) -> 'a3 **)
+
+      let fold_rec_bis f i m pmorphism pempty pstep =
+        fold_rec f i m (fun m0 _ -> pmorphism TE.empty m0 i __ pempty)
+          (fun k e a m' m'' _ _ _ x ->
+          pmorphism (TE.add k e m') m'' (f k e a) __ (pstep k e a m' __ __ x))
+
+      (** val fold_rec_nodep :
+          (TE.key -> 'a1 -> 'a2 -> 'a2) -> 'a2 -> 'a1 TE.t -> 'a3 -> (TE.key
+          -> 'a1 -> 'a2 -> __ -> 'a3 -> 'a3) -> 'a3 **)
+
+      let fold_rec_nodep f i m x x0 =
+        fold_rec_bis f i m (fun _ _ _ _ x1 -> x1) x (fun k e a _ _ _ x1 ->
+          x0 k e a __ x1)
+
+      (** val fold_rec_weak :
+          (TE.key -> 'a1 -> 'a2 -> 'a2) -> 'a2 -> ('a1 TE.t -> 'a1 TE.t ->
+          'a2 -> __ -> 'a3 -> 'a3) -> 'a3 -> (TE.key -> 'a1 -> 'a2 -> 'a1
+          TE.t -> __ -> 'a3 -> 'a3) -> 'a1 TE.t -> 'a3 **)
+
+      let fold_rec_weak f i x x0 x1 m =
+        fold_rec_bis f i m x x0 (fun k e a m' _ _ x2 -> x1 k e a m' __ x2)
+
+      (** val fold_rel :
+          (TE.key -> 'a1 -> 'a2 -> 'a2) -> (TE.key -> 'a1 -> 'a3 -> 'a3) ->
+          'a2 -> 'a3 -> 'a1 TE.t -> 'a4 -> (TE.key -> 'a1 -> 'a2 -> 'a3 -> __
+          -> 'a4 -> 'a4) -> 'a4 **)
+
+      let fold_rel f g i j m rempty rstep =
+        let l = rev (TE.elements m) in
+        let rstep' = fun k e a b x -> rstep k e a b __ x in
+        let rec f0 l0 rstep'0 =
+          match l0 with
+          | [] -> rempty
+          | y :: l1 ->
+            rstep'0 (fst y) (snd y) (fold_right (uncurry f) i l1)
+              (fold_right (uncurry g) j l1) __
+              (f0 l1 (fun k e a0 b _ x -> rstep'0 k e a0 b __ x))
+        in f0 l (fun k e a b _ x -> rstep' k e a b x)
+
+      (** val map_induction :
+          ('a1 TE.t -> __ -> 'a2) -> ('a1 TE.t -> 'a1 TE.t -> 'a2 -> TE.key
+          -> 'a1 -> __ -> __ -> 'a2) -> 'a1 TE.t -> 'a2 **)
+
+      let map_induction x x0 m =
+        fold_rec (fun _ _ _ -> ()) () m x (fun k e _ m' m'' _ _ _ x1 ->
+          x0 m' m'' x1 k e __ __)
+
+      (** val map_induction_bis :
+          ('a1 TE.t -> 'a1 TE.t -> __ -> 'a2 -> 'a2) -> 'a2 -> (TE.key -> 'a1
+          -> 'a1 TE.t -> __ -> 'a2 -> 'a2) -> 'a1 TE.t -> 'a2 **)
+
+      let map_induction_bis x x0 x1 m =
+        fold_rec_bis (fun _ _ _ -> ()) () m (fun m0 m' _ _ x2 ->
+          x m0 m' __ x2) x0 (fun k e _ m' _ _ x2 -> x1 k e m' __ x2)
+
+      (** val cardinal_inv_2 : 'a1 TE.t -> int -> (TE.key * 'a1) **)
+
+      let cardinal_inv_2 m _ =
+        let l = TE.elements m in
+        (match l with
+         | [] -> assert false (* absurd case *)
+         | a :: _ -> a)
+
+      (** val cardinal_inv_2b : 'a1 TE.t -> (TE.key * 'a1) **)
+
+      let cardinal_inv_2b m =
+        let n = TE.cardinal m in
+        let x = fun x -> cardinal_inv_2 m x in
+        ((fun fO fS n -> if n=0 then fO () else fS (n-1))
+           (fun _ -> assert false (* absurd case *))
+           (fun n0 -> x n0)
+           n)
+
+      (** val filter : (TE.key -> 'a1 -> bool) -> 'a1 TE.t -> 'a1 TE.t **)
+
+      let filter f m =
+        TE.fold (fun k e m0 -> if f k e then TE.add k e m0 else m0) m TE.empty
+
+      (** val for_all : (TE.key -> 'a1 -> bool) -> 'a1 TE.t -> bool **)
+
+      let for_all f m =
+        TE.fold (fun k e b -> if f k e then b else false) m true
+
+      (** val exists_ : (TE.key -> 'a1 -> bool) -> 'a1 TE.t -> bool **)
+
+      let exists_ f m =
+        TE.fold (fun k e b -> if f k e then true else b) m false
+
+      (** val partition :
+          (TE.key -> 'a1 -> bool) -> 'a1 TE.t -> 'a1 TE.t * 'a1 TE.t **)
+
+      let partition f m =
+        ((filter f m), (filter (fun k e -> negb (f k e)) m))
+
+      (** val update : 'a1 TE.t -> 'a1 TE.t -> 'a1 TE.t **)
+
+      let update m1 m2 =
+        TE.fold TE.add m2 m1
+
+      (** val restrict : 'a1 TE.t -> 'a1 TE.t -> 'a1 TE.t **)
+
+      let restrict m1 m2 =
+        filter (fun k _ -> TE.mem k m2) m1
+
+      (** val diff : 'a1 TE.t -> 'a1 TE.t -> 'a1 TE.t **)
+
+      let diff m1 m2 =
+        filter (fun k _ -> negb (TE.mem k m2)) m1
+
+      (** val coq_Partition_In :
+          'a1 TE.t -> 'a1 TE.t -> 'a1 TE.t -> TE.key -> bool **)
+
+      let coq_Partition_In _ m1 _ k =
+        F.coq_In_dec m1 k
+
+      (** val update_dec : 'a1 TE.t -> 'a1 TE.t -> TE.key -> 'a1 -> bool **)
+
+      let update_dec _ m' k _ =
+        F.coq_In_dec m' k
+
+      (** val filter_dom : (TE.key -> bool) -> 'a1 TE.t -> 'a1 TE.t **)
+
+      let filter_dom f =
+        filter (fun k _ -> f k)
+
+      (** val filter_range : ('a1 -> bool) -> 'a1 TE.t -> 'a1 TE.t **)
+
+      let filter_range f =
+        filter (fun _ -> f)
+
+      (** val for_all_dom : (TE.key -> bool) -> 'a1 TE.t -> bool **)
+
+      let for_all_dom f =
+        for_all (fun k _ -> f k)
+
+      (** val for_all_range : ('a1 -> bool) -> 'a1 TE.t -> bool **)
+
+      let for_all_range f =
+        for_all (fun _ -> f)
+
+      (** val exists_dom : (TE.key -> bool) -> 'a1 TE.t -> bool **)
+
+      let exists_dom f =
+        exists_ (fun k _ -> f k)
+
+      (** val exists_range : ('a1 -> bool) -> 'a1 TE.t -> bool **)
+
+      let exists_range f =
+        exists_ (fun _ -> f)
+
+      (** val partition_dom :
+          (TE.key -> bool) -> 'a1 TE.t -> 'a1 TE.t * 'a1 TE.t **)
+
+      let partition_dom f =
+        partition (fun k _ -> f k)
+
+      (** val partition_range :
+          ('a1 -> bool) -> 'a1 TE.t -> 'a1 TE.t * 'a1 TE.t **)
+
+      let partition_range f =
+        partition (fun _ -> f)
+     end
+
+    (** val gtb : (TE.key * 'a1) -> (TE.key * 'a1) -> bool **)
+
+    let gtb p p' =
+      match TE.E.compare (fst p) (fst p') with
+      | OrderedType.GT -> true
+      | _ -> false
+
+    (** val leb : (TE.key * 'a1) -> (TE.key * 'a1) -> bool **)
+
+    let leb p p' =
+      negb (gtb p p')
+
+    (** val elements_lt :
+        (TE.key * 'a1) -> 'a1 TE.t -> (TE.key * 'a1) list **)
+
+    let elements_lt p m =
+      filter (gtb p) (TE.elements m)
+
+    (** val elements_ge :
+        (TE.key * 'a1) -> 'a1 TE.t -> (TE.key * 'a1) list **)
+
+    let elements_ge p m =
+      filter (leb p) (TE.elements m)
+
+    (** val max_elt_aux : (TE.key * 'a1) list -> (TE.key * 'a1) option **)
+
+    let rec max_elt_aux = function
+    | [] -> None
+    | p :: l0 -> (match l0 with
+                  | [] -> Some p
+                  | _ :: _ -> max_elt_aux l0)
+
+    (** val max_elt : 'a1 TE.t -> (TE.key * 'a1) option **)
+
+    let max_elt m =
+      max_elt_aux (TE.elements m)
+
+    (** val min_elt : 'a1 TE.t -> (TE.key * 'a1) option **)
+
+    let min_elt m =
+      match TE.elements m with
+      | [] -> None
+      | p :: _ -> Some p
+
+    (** val map_induction_max :
+        ('a1 TE.t -> __ -> 'a2) -> ('a1 TE.t -> 'a1 TE.t -> 'a2 -> TE.SE.t ->
+        'a1 -> __ -> __ -> 'a2) -> 'a1 TE.t -> 'a2 **)
+
+    let map_induction_max x x0 m =
+      let n = TE.cardinal m in
+      let rec f n0 m0 =
+        (fun fO fS n -> if n=0 then fO () else fS (n-1))
+          (fun _ -> x m0 __)
+          (fun n1 ->
+          match max_elt m0 with
+          | Some a ->
+            let (a0, b) = a in
+            x0 (TE.remove a0 m0) m0 (f n1 (TE.remove a0 m0)) a0 b __ __
+          | None -> x m0 __)
+          n0
+      in f n m
+
+    (** val map_induction_min :
+        ('a1 TE.t -> __ -> 'a2) -> ('a1 TE.t -> 'a1 TE.t -> 'a2 -> TE.SE.t ->
+        'a1 -> __ -> __ -> 'a2) -> 'a1 TE.t -> 'a2 **)
+
+    let map_induction_min x x0 m =
+      let n = TE.cardinal m in
+      let rec f n0 m0 =
+        (fun fO fS n -> if n=0 then fO () else fS (n-1))
+          (fun _ -> x m0 __)
+          (fun n1 ->
+          match min_elt m0 with
+          | Some a ->
+            let (a0, b) = a in
+            x0 (TE.remove a0 m0) m0 (f n1 (TE.remove a0 m0)) a0 b __ __
+          | None -> x m0 __)
+          n0
+      in f n m
+   end
+
+  (** val eqb : TE.SE.t -> TE.SE.t -> bool **)
+
+  let eqb x y =
+    if TE.E.eq_dec x y then true else false
+
+  (** val coq_In_dec : 'a1 TE.t -> TE.key -> bool **)
+
+  let coq_In_dec =
+    F.coq_In_dec
+
+  module ME = OP.ME
+
+  module O = OP.O
+
+  module P = OP.P
+
+  (** val gtb : (TE.key * 'a1) -> (TE.key * 'a1) -> bool **)
+
+  let gtb p p' =
+    match TE.E.compare (fst p) (fst p') with
+    | OrderedType.GT -> true
+    | _ -> false
+
+  (** val leb : (TE.key * 'a1) -> (TE.key * 'a1) -> bool **)
+
+  let leb p p' =
+    negb (gtb p p')
+
+  (** val elements_lt : (TE.key * 'a1) -> 'a1 TE.t -> (TE.key * 'a1) list **)
+
+  let elements_lt p m =
+    filter (gtb p) (TE.elements m)
+
+  (** val elements_ge : (TE.key * 'a1) -> 'a1 TE.t -> (TE.key * 'a1) list **)
+
+  let elements_ge p m =
+    filter (leb p) (TE.elements m)
+
+  (** val max_elt_aux : (TE.key * 'a1) list -> (TE.key * 'a1) option **)
+
+  let rec max_elt_aux = function
+  | [] -> None
+  | p :: l0 -> (match l0 with
+                | [] -> Some p
+                | _ :: _ -> max_elt_aux l0)
+
+  (** val max_elt : 'a1 TE.t -> (TE.key * 'a1) option **)
+
+  let max_elt m =
+    max_elt_aux (TE.elements m)
+
+  (** val min_elt : 'a1 TE.t -> (TE.key * 'a1) option **)
+
+  let min_elt m =
+    match TE.elements m with
+    | [] -> None
+    | p :: _ -> Some p
+
+  (** val map_induction_max :
+      ('a1 TE.t -> __ -> 'a2) -> ('a1 TE.t -> 'a1 TE.t -> 'a2 -> TE.SE.t ->
+      'a1 -> __ -> __ -> 'a2) -> 'a1 TE.t -> 'a2 **)
+
+  let map_induction_max =
+    OP.map_induction_max
+
+  (** val map_induction_min :
+      ('a1 TE.t -> __ -> 'a2) -> ('a1 TE.t -> 'a1 TE.t -> 'a2 -> TE.SE.t ->
+      'a1 -> __ -> __ -> 'a2) -> 'a1 TE.t -> 'a2 **)
+
+  let map_induction_min =
+    OP.map_induction_min
+
+  (** val memP : TE.key -> 'a1 TE.t -> reflect **)
+
+  let memP k m =
+    let _evar_0_ = fun _ -> ReflectT in
+    let _evar_0_0 = fun _ -> ReflectF in
+    if TE.mem k m then _evar_0_ __ else _evar_0_0 __
+
+  (** val split : ('a1 * 'a2) TE.t -> 'a1 TE.t * 'a2 TE.t **)
+
+  let split m =
+    ((TE.fold (fun k e m1 -> TE.add k (fst e) m1) m TE.empty),
+      (TE.fold (fun k e m2 -> TE.add k (snd e) m2) m TE.empty))
+
+  module EFacts = OrderedType.OrderedTypeFacts(TE.E)
+
+  (** val max_opt : TE.key -> TE.key option -> TE.key **)
+
+  let max_opt k = function
+  | Some k' -> (match TE.E.compare k k' with
+                | OrderedType.LT -> k'
+                | _ -> k)
+  | None -> k
+
+  (** val max_key_elements : (TE.key * 'a1) list -> TE.key option **)
+
+  let rec max_key_elements = function
+  | [] -> None
+  | p :: tl -> let (k, _) = p in Some (max_opt k (max_key_elements tl))
+
+  (** val max_key : 'a1 TE.t -> TE.key option **)
+
+  let max_key m =
+    max_key_elements (TE.elements m)
+
+  (** val min_opt : TE.key -> TE.key option -> TE.key **)
+
+  let min_opt k = function
+  | Some k' -> (match TE.E.compare k k' with
+                | OrderedType.GT -> k'
+                | _ -> k)
+  | None -> k
+
+  (** val min_key_elements : (TE.key * 'a1) list -> TE.key option **)
+
+  let rec min_key_elements = function
+  | [] -> None
+  | p :: tl -> let (k, _) = p in Some (min_opt k (min_key_elements tl))
+
+  (** val min_key : 'a1 TE.t -> TE.key option **)
+
+  let min_key m =
+    min_key_elements (TE.elements m)
+
+  (** val equalP : typ TE.t -> typ TE.t -> reflect **)
+
+  let equalP x y =
+    ssr_have __ (fun _ ->
+      let _evar_0_ = fun _ -> ReflectT in
+      let _evar_0_0 = fun _ -> ReflectF in
+      if TE.equal typ_eqn x y then _evar_0_ __ else _evar_0_0 __)
+
+  (** val eequalP : typ TE.t -> typ TE.t -> reflect **)
+
+  let eequalP =
+    equalP
  end
 
 module MakeTypEnv =
@@ -151,6 +617,11 @@ module MakeTypEnv =
 
   let vsize v e =
     sizeof_typ (vtyp v e)
+
+  (** val eequal : typ t -> typ t -> bool **)
+
+  let eequal =
+    equal typ_eqn
  end
 
 module SSATE = MakeTypEnv(SSAVarOrder)(SSAVM)
