src/ocaml/extraction/TypEnv.mli
@@ -1,7 +1,10 @@
 open Bool
+open Datatypes
 open FMaps
+open List0
 open Typ
 open Var
+open Ssreflect
 
 type __ = Obj.t
 
@@ -51,6 +54,380 @@ module type TypEnv =
   val vtyp : SE.t -> env -> typ
 
   val vsize : SE.t -> env -> int
+
+  val eequal : env -> env -> bool
+ end
+
+module TypEnvLemmas :
+ functor (TE:TypEnv) ->
+ sig
+  module F :
+   sig
+    val eqb : TE.SE.t -> TE.SE.t -> bool
+
+    val coq_In_dec : 'a1 TE.t -> TE.key -> bool
+   end
+
+  module OP :
+   sig
+    module ME :
+     sig
+      module TO :
+       sig
+        type t = TE.SE.t
+       end
+
+      module IsTO :
+       sig
+       end
+
+      module OrderTac :
+       sig
+       end
+
+      val eq_dec : TE.SE.t -> TE.SE.t -> bool
+
+      val lt_dec : TE.SE.t -> TE.SE.t -> bool
+
+      val eqb : TE.SE.t -> TE.SE.t -> bool
+     end
+
+    module O :
+     sig
+      module MO :
+       sig
+        module TO :
+         sig
+          type t = TE.SE.t
+         end
+
+        module IsTO :
+         sig
+         end
+
+        module OrderTac :
+         sig
+         end
+
+        val eq_dec : TE.SE.t -> TE.SE.t -> bool
+
+        val lt_dec : TE.SE.t -> TE.SE.t -> bool
+
+        val eqb : TE.SE.t -> TE.SE.t -> bool
+       end
+     end
+
+    module P :
+     sig
+      module F :
+       sig
+        val eqb : TE.SE.t -> TE.SE.t -> bool
+
+        val coq_In_dec : 'a1 TE.t -> TE.key -> bool
+       end
+
+      val uncurry : ('a1 -> 'a2 -> 'a3) -> ('a1 * 'a2) -> 'a3
+
+      val of_list : (TE.key * 'a1) list -> 'a1 TE.t
+
+      val to_list : 'a1 TE.t -> (TE.key * 'a1) list
+
+      val fold_rec :
+        (TE.key -> 'a1 -> 'a2 -> 'a2) -> 'a2 -> 'a1 TE.t -> ('a1 TE.t -> __
+        -> 'a3) -> (TE.key -> 'a1 -> 'a2 -> 'a1 TE.t -> 'a1 TE.t -> __ -> __
+        -> __ -> 'a3 -> 'a3) -> 'a3
+
+      val fold_rec_bis :
+        (TE.key -> 'a1 -> 'a2 -> 'a2) -> 'a2 -> 'a1 TE.t -> ('a1 TE.t -> 'a1
+        TE.t -> 'a2 -> __ -> 'a3 -> 'a3) -> 'a3 -> (TE.key -> 'a1 -> 'a2 ->
+        'a1 TE.t -> __ -> __ -> 'a3 -> 'a3) -> 'a3
+
+      val fold_rec_nodep :
+        (TE.key -> 'a1 -> 'a2 -> 'a2) -> 'a2 -> 'a1 TE.t -> 'a3 -> (TE.key ->
+        'a1 -> 'a2 -> __ -> 'a3 -> 'a3) -> 'a3
+
+      val fold_rec_weak :
+        (TE.key -> 'a1 -> 'a2 -> 'a2) -> 'a2 -> ('a1 TE.t -> 'a1 TE.t -> 'a2
+        -> __ -> 'a3 -> 'a3) -> 'a3 -> (TE.key -> 'a1 -> 'a2 -> 'a1 TE.t ->
+        __ -> 'a3 -> 'a3) -> 'a1 TE.t -> 'a3
+
+      val fold_rel :
+        (TE.key -> 'a1 -> 'a2 -> 'a2) -> (TE.key -> 'a1 -> 'a3 -> 'a3) -> 'a2
+        -> 'a3 -> 'a1 TE.t -> 'a4 -> (TE.key -> 'a1 -> 'a2 -> 'a3 -> __ ->
+        'a4 -> 'a4) -> 'a4
+
+      val map_induction :
+        ('a1 TE.t -> __ -> 'a2) -> ('a1 TE.t -> 'a1 TE.t -> 'a2 -> TE.key ->
+        'a1 -> __ -> __ -> 'a2) -> 'a1 TE.t -> 'a2
+
+      val map_induction_bis :
+        ('a1 TE.t -> 'a1 TE.t -> __ -> 'a2 -> 'a2) -> 'a2 -> (TE.key -> 'a1
+        -> 'a1 TE.t -> __ -> 'a2 -> 'a2) -> 'a1 TE.t -> 'a2
+
+      val cardinal_inv_2 : 'a1 TE.t -> int -> (TE.key * 'a1)
+
+      val cardinal_inv_2b : 'a1 TE.t -> (TE.key * 'a1)
+
+      val filter : (TE.key -> 'a1 -> bool) -> 'a1 TE.t -> 'a1 TE.t
+
+      val for_all : (TE.key -> 'a1 -> bool) -> 'a1 TE.t -> bool
+
+      val exists_ : (TE.key -> 'a1 -> bool) -> 'a1 TE.t -> bool
+
+      val partition :
+        (TE.key -> 'a1 -> bool) -> 'a1 TE.t -> 'a1 TE.t * 'a1 TE.t
+
+      val update : 'a1 TE.t -> 'a1 TE.t -> 'a1 TE.t
+
+      val restrict : 'a1 TE.t -> 'a1 TE.t -> 'a1 TE.t
+
+      val diff : 'a1 TE.t -> 'a1 TE.t -> 'a1 TE.t
+
+      val coq_Partition_In :
+        'a1 TE.t -> 'a1 TE.t -> 'a1 TE.t -> TE.key -> bool
+
+      val update_dec : 'a1 TE.t -> 'a1 TE.t -> TE.key -> 'a1 -> bool
+
+      val filter_dom : (TE.key -> bool) -> 'a1 TE.t -> 'a1 TE.t
+
+      val filter_range : ('a1 -> bool) -> 'a1 TE.t -> 'a1 TE.t
+
+      val for_all_dom : (TE.key -> bool) -> 'a1 TE.t -> bool
+
+      val for_all_range : ('a1 -> bool) -> 'a1 TE.t -> bool
+
+      val exists_dom : (TE.key -> bool) -> 'a1 TE.t -> bool
+
+      val exists_range : ('a1 -> bool) -> 'a1 TE.t -> bool
+
+      val partition_dom : (TE.key -> bool) -> 'a1 TE.t -> 'a1 TE.t * 'a1 TE.t
+
+      val partition_range : ('a1 -> bool) -> 'a1 TE.t -> 'a1 TE.t * 'a1 TE.t
+     end
+
+    val gtb : (TE.key * 'a1) -> (TE.key * 'a1) -> bool
+
+    val leb : (TE.key * 'a1) -> (TE.key * 'a1) -> bool
+
+    val elements_lt : (TE.key * 'a1) -> 'a1 TE.t -> (TE.key * 'a1) list
+
+    val elements_ge : (TE.key * 'a1) -> 'a1 TE.t -> (TE.key * 'a1) list
+
+    val max_elt_aux : (TE.key * 'a1) list -> (TE.key * 'a1) option
+
+    val max_elt : 'a1 TE.t -> (TE.key * 'a1) option
+
+    val min_elt : 'a1 TE.t -> (TE.key * 'a1) option
+
+    val map_induction_max :
+      ('a1 TE.t -> __ -> 'a2) -> ('a1 TE.t -> 'a1 TE.t -> 'a2 -> TE.SE.t ->
+      'a1 -> __ -> __ -> 'a2) -> 'a1 TE.t -> 'a2
+
+    val map_induction_min :
+      ('a1 TE.t -> __ -> 'a2) -> ('a1 TE.t -> 'a1 TE.t -> 'a2 -> TE.SE.t ->
+      'a1 -> __ -> __ -> 'a2) -> 'a1 TE.t -> 'a2
+   end
+
+  val eqb : TE.SE.t -> TE.SE.t -> bool
+
+  val coq_In_dec : 'a1 TE.t -> TE.key -> bool
+
+  module ME :
+   sig
+    module TO :
+     sig
+      type t = TE.SE.t
+     end
+
+    module IsTO :
+     sig
+     end
+
+    module OrderTac :
+     sig
+     end
+
+    val eq_dec : TE.SE.t -> TE.SE.t -> bool
+
+    val lt_dec : TE.SE.t -> TE.SE.t -> bool
+
+    val eqb : TE.SE.t -> TE.SE.t -> bool
+   end
+
+  module O :
+   sig
+    module MO :
+     sig
+      module TO :
+       sig
+        type t = TE.SE.t
+       end
+
+      module IsTO :
+       sig
+       end
+
+      module OrderTac :
+       sig
+       end
+
+      val eq_dec : TE.SE.t -> TE.SE.t -> bool
+
+      val lt_dec : TE.SE.t -> TE.SE.t -> bool
+
+      val eqb : TE.SE.t -> TE.SE.t -> bool
+     end
+   end
+
+  module P :
+   sig
+    module F :
+     sig
+      val eqb : TE.SE.t -> TE.SE.t -> bool
+
+      val coq_In_dec : 'a1 TE.t -> TE.key -> bool
+     end
+
+    val uncurry : ('a1 -> 'a2 -> 'a3) -> ('a1 * 'a2) -> 'a3
+
+    val of_list : (TE.key * 'a1) list -> 'a1 TE.t
+
+    val to_list : 'a1 TE.t -> (TE.key * 'a1) list
+
+    val fold_rec :
+      (TE.key -> 'a1 -> 'a2 -> 'a2) -> 'a2 -> 'a1 TE.t -> ('a1 TE.t -> __ ->
+      'a3) -> (TE.key -> 'a1 -> 'a2 -> 'a1 TE.t -> 'a1 TE.t -> __ -> __ -> __
+      -> 'a3 -> 'a3) -> 'a3
+
+    val fold_rec_bis :
+      (TE.key -> 'a1 -> 'a2 -> 'a2) -> 'a2 -> 'a1 TE.t -> ('a1 TE.t -> 'a1
+      TE.t -> 'a2 -> __ -> 'a3 -> 'a3) -> 'a3 -> (TE.key -> 'a1 -> 'a2 -> 'a1
+      TE.t -> __ -> __ -> 'a3 -> 'a3) -> 'a3
+
+    val fold_rec_nodep :
+      (TE.key -> 'a1 -> 'a2 -> 'a2) -> 'a2 -> 'a1 TE.t -> 'a3 -> (TE.key ->
+      'a1 -> 'a2 -> __ -> 'a3 -> 'a3) -> 'a3
+
+    val fold_rec_weak :
+      (TE.key -> 'a1 -> 'a2 -> 'a2) -> 'a2 -> ('a1 TE.t -> 'a1 TE.t -> 'a2 ->
+      __ -> 'a3 -> 'a3) -> 'a3 -> (TE.key -> 'a1 -> 'a2 -> 'a1 TE.t -> __ ->
+      'a3 -> 'a3) -> 'a1 TE.t -> 'a3
+
+    val fold_rel :
+      (TE.key -> 'a1 -> 'a2 -> 'a2) -> (TE.key -> 'a1 -> 'a3 -> 'a3) -> 'a2
+      -> 'a3 -> 'a1 TE.t -> 'a4 -> (TE.key -> 'a1 -> 'a2 -> 'a3 -> __ -> 'a4
+      -> 'a4) -> 'a4
+
+    val map_induction :
+      ('a1 TE.t -> __ -> 'a2) -> ('a1 TE.t -> 'a1 TE.t -> 'a2 -> TE.key ->
+      'a1 -> __ -> __ -> 'a2) -> 'a1 TE.t -> 'a2
+
+    val map_induction_bis :
+      ('a1 TE.t -> 'a1 TE.t -> __ -> 'a2 -> 'a2) -> 'a2 -> (TE.key -> 'a1 ->
+      'a1 TE.t -> __ -> 'a2 -> 'a2) -> 'a1 TE.t -> 'a2
+
+    val cardinal_inv_2 : 'a1 TE.t -> int -> (TE.key * 'a1)
+
+    val cardinal_inv_2b : 'a1 TE.t -> (TE.key * 'a1)
+
+    val filter : (TE.key -> 'a1 -> bool) -> 'a1 TE.t -> 'a1 TE.t
+
+    val for_all : (TE.key -> 'a1 -> bool) -> 'a1 TE.t -> bool
+
+    val exists_ : (TE.key -> 'a1 -> bool) -> 'a1 TE.t -> bool
+
+    val partition : (TE.key -> 'a1 -> bool) -> 'a1 TE.t -> 'a1 TE.t * 'a1 TE.t
+
+    val update : 'a1 TE.t -> 'a1 TE.t -> 'a1 TE.t
+
+    val restrict : 'a1 TE.t -> 'a1 TE.t -> 'a1 TE.t
+
+    val diff : 'a1 TE.t -> 'a1 TE.t -> 'a1 TE.t
+
+    val coq_Partition_In : 'a1 TE.t -> 'a1 TE.t -> 'a1 TE.t -> TE.key -> bool
+
+    val update_dec : 'a1 TE.t -> 'a1 TE.t -> TE.key -> 'a1 -> bool
+
+    val filter_dom : (TE.key -> bool) -> 'a1 TE.t -> 'a1 TE.t
+
+    val filter_range : ('a1 -> bool) -> 'a1 TE.t -> 'a1 TE.t
+
+    val for_all_dom : (TE.key -> bool) -> 'a1 TE.t -> bool
+
+    val for_all_range : ('a1 -> bool) -> 'a1 TE.t -> bool
+
+    val exists_dom : (TE.key -> bool) -> 'a1 TE.t -> bool
+
+    val exists_range : ('a1 -> bool) -> 'a1 TE.t -> bool
+
+    val partition_dom : (TE.key -> bool) -> 'a1 TE.t -> 'a1 TE.t * 'a1 TE.t
+
+    val partition_range : ('a1 -> bool) -> 'a1 TE.t -> 'a1 TE.t * 'a1 TE.t
+   end
+
+  val gtb : (TE.key * 'a1) -> (TE.key * 'a1) -> bool
+
+  val leb : (TE.key * 'a1) -> (TE.key * 'a1) -> bool
+
+  val elements_lt : (TE.key * 'a1) -> 'a1 TE.t -> (TE.key * 'a1) list
+
+  val elements_ge : (TE.key * 'a1) -> 'a1 TE.t -> (TE.key * 'a1) list
+
+  val max_elt_aux : (TE.key * 'a1) list -> (TE.key * 'a1) option
+
+  val max_elt : 'a1 TE.t -> (TE.key * 'a1) option
+
+  val min_elt : 'a1 TE.t -> (TE.key * 'a1) option
+
+  val map_induction_max :
+    ('a1 TE.t -> __ -> 'a2) -> ('a1 TE.t -> 'a1 TE.t -> 'a2 -> TE.SE.t -> 'a1
+    -> __ -> __ -> 'a2) -> 'a1 TE.t -> 'a2
+
+  val map_induction_min :
+    ('a1 TE.t -> __ -> 'a2) -> ('a1 TE.t -> 'a1 TE.t -> 'a2 -> TE.SE.t -> 'a1
+    -> __ -> __ -> 'a2) -> 'a1 TE.t -> 'a2
+
+  val memP : TE.key -> 'a1 TE.t -> reflect
+
+  val split : ('a1 * 'a2) TE.t -> 'a1 TE.t * 'a2 TE.t
+
+  module EFacts :
+   sig
+    module TO :
+     sig
+      type t = TE.SE.t
+     end
+
+    module IsTO :
+     sig
+     end
+
+    module OrderTac :
+     sig
+     end
+
+    val eq_dec : TE.SE.t -> TE.SE.t -> bool
+
+    val lt_dec : TE.SE.t -> TE.SE.t -> bool
+
+    val eqb : TE.SE.t -> TE.SE.t -> bool
+   end
+
+  val max_opt : TE.key -> TE.key option -> TE.key
+
+  val max_key_elements : (TE.key * 'a1) list -> TE.key option
+
+  val max_key : 'a1 TE.t -> TE.key option
+
+  val min_opt : TE.key -> TE.key option -> TE.key
+
+  val min_key_elements : (TE.key * 'a1) list -> TE.key option
+
+  val min_key : 'a1 TE.t -> TE.key option
+
+  val equalP : typ TE.t -> typ TE.t -> reflect
+
+  val eequalP : typ TE.t -> typ TE.t -> reflect
  end
 
 module MakeTypEnv :
@@ -471,6 +848,8 @@ module MakeTypEnv :
   val vtyp : V.t -> env -> typ
 
   val vsize : V.t -> env -> int
+
+  val eequal : typ t -> typ t -> bool
  end
 
 module SSATE :
@@ -901,4 +1280,6 @@ module SSATE :
   val vtyp : SSAVarOrder.t -> env -> typ
 
   val vsize : SSAVarOrder.t -> env -> int
+
+  val eequal : typ t -> typ t -> bool
  end
